Add set_op

dataplane/Examples/Batch_op_Correctness.thy
@@ -7,561 +7,19 @@ imports
   "../MyProduct_Instances"
   "../AntichainOrder"
    Dataplane.LList_Haskell_Setup
-  Traces_op
+  Set_op
+  Source_op
 begin
 
-partial_function (llist) batch_fun_spec where
- "batch_fun_spec f buf caps lxs = (case lxs of
-    LNil \<Rightarrow> (
-    let compl_batches = (\<lambda> t. map fst ((filter (\<lambda> (d, t'). t' = t)) buf)) in
-    let outs =  map (\<lambda> t. map (\<lambda> x. (x, t)) (f (compl_batches t))) (rmdups {} (map snd buf)) in
-    llist_of outs)
-  | LCons (Data t (d :: 'd1)) lxs' \<Rightarrow> batch_fun_spec f ((d, t) # buf) caps lxs'
-  | LCons (Mint t) lxs' \<Rightarrow> batch_fun_spec f buf (caps @ [t]) lxs'
-  | LCons (Drop t) lxs' \<Rightarrow> (
-    let below_caps = filter (\<lambda> t'. \<not> frontier_less_equal (frontier (zmset_of (mset caps - {# t #}))) t') (rmdups {} (map snd buf)) in
-    let compl_batches = (\<lambda> t. map fst (filter (\<lambda> (d, t'). t' = t \<and> t' \<in> set below_caps) buf)) in
-    let outs = concat (map (\<lambda> t. map (\<lambda> x. (x, t)) (f (compl_batches t))) (filter (\<lambda> t. t \<in> set below_caps) (rmdups {} (map snd buf)))) in
-    let buf' = filter (\<lambda> (d, t). t \<notin> set below_caps) buf in
-    LCons outs (batch_fun_spec f buf' (remove1 t caps) lxs')))"
-
-fun foo where
- "foo f lxs buf caps = (case lxs of
-    [] \<Rightarrow> (
-    let below_caps = filter (\<lambda> t'. \<not> frontier_less_equal (frontier (zmset_of (mset caps))) t') (rmdups {} (map snd buf)) in
-    let compl_batches = (\<lambda> t. map fst (filter (\<lambda> (d, t'). t' = t \<and> t' \<in> set below_caps) buf)) in
-    let outs = concat (map (\<lambda> t. map (\<lambda> x. (x, t)) (f (compl_batches t))) (filter (\<lambda> t. t \<in> set below_caps) (rmdups {} (map snd buf)))) in
-    let buf' = filter (\<lambda> (d, t). t \<notin> set below_caps) buf in
-    (outs, buf', caps))
-  | (Data t (d :: 'd1)) # lxs' \<Rightarrow> foo f lxs' ((d, t) # buf) caps
-  | (Mint t) # lxs' \<Rightarrow> foo f lxs' buf (caps @ [t])
-  | (Drop t) # lxs' \<Rightarrow> foo f lxs' buf (remove1 t caps))"
-
-declare batch_fun_spec.simps[code]
-
-(* filter cUNIV to not have empty outputs*)
-corec spec_op where
-  "spec_op m (f :: 'a list \<Rightarrow> 'b list) lxs buf caps outp = choice2
-   (Choice ((cimage (\<lambda> n. 
-     let (outs, buf', caps') = foo f (ltaken n lxs) buf caps in
-     (case outp @ outs of x # xs \<Rightarrow> (Write (spec_op m f (ldropn n lxs) buf' caps' xs) 1 x))) (
-      cfilter (\<lambda> n. fst (foo f (ltaken n lxs) buf caps) \<noteq> [])
-      (cset_of_llist (llist_of ([0..< Suc m])))))))
-    (case outp of 
-       [] \<Rightarrow> \<oslash>
-     | x # xs \<Rightarrow> Write (spec_op m f lxs buf caps xs) 1 x)"
 
 abbreviation "t0 \<equiv> MyPair (0 :: nat) (0 :: nat)"
 abbreviation "t_1_0 \<equiv> MyPair (Suc 0) (0 :: nat)"
 abbreviation "t_0_1 \<equiv> MyPair (0 :: nat) (Suc 0)"
 abbreviation "t_1_1 \<equiv> MyPair (Suc 0) (Suc 0)"
 
-lemma t0_is_bot[simp]:
-  "\<bottom> = MyPair (0 :: nat) (0 :: nat)"
-  by (simp add: bot_myprod_def bot_nat_def)
-
-abbreviation "inps1 \<equiv> llist_of [Mint 1, Data 1 44, Data 1 6, Data (0 :: nat) (0 :: nat), Data 0 42, Drop 0, Data 1 43]"
-
 abbreviation "list_inps2 \<equiv> 
  [Mint t_1_0, Mint t_0_1, Mint t_1_1, Drop t0, Data t_1_1 10, Drop t_1_1, Data t_0_1 7, Data t_1_0 (3 :: nat), Drop t_1_0, Drop t_0_1]"
-
-value "[frontier {# t0, t_1_1, t_1_0, t_0_1 #}\<^sub>z, frontier {# t_1_1, t_1_0, t_0_1 #}\<^sub>z, frontier {# t_1_0, t_0_1 #}\<^sub>z, frontier {# t_0_1 #}\<^sub>z, frontier {#}\<^sub>z] "
-value "[frontier {# t0, t_1_1, t_1_0, t_0_1 #}\<^sub>z, frontier {# t_1_0, t_0_1 #}\<^sub>z, frontier {# t_0_1 #}\<^sub>z, frontier {#}\<^sub>z] "
-value "[frontier {# t0, t_1_1, t_1_0, t_0_1 #}\<^sub>z, frontier {# t_0_1 #}\<^sub>z, frontier {#}\<^sub>z] "
-value "[frontier {# t0, t_1_1, t_1_0, t_0_1 #}\<^sub>z, frontier {#}\<^sub>z] "
-
 abbreviation "inps2 \<equiv> llist_of list_inps2"
-
-abbreviation \<open>r1 \<equiv> lconcat (batch_fun_spec (\<lambda> b. [Max (set b)]) [] [\<bottom>] inps1)\<close>
-value r1
-
-abbreviation \<open>r2 \<equiv> lconcat (batch_fun_spec (\<lambda> b. [Max (set b)]) [] [\<bottom>] inps2)\<close>
-value r2
-
-abbreviation "spec_op_test \<equiv> (spec_op (length list_inps2) (\<lambda> b. [Max (set b)]) inps2 [] [\<bottom>] []) :: (1, 1, nat \<times> (nat, nat) myprod) op"
-
-
-record ('nid, 'p, 't, 'd) dataplane_state =
-  ecaps :: "('nid, 'p) location \<Rightarrow> 't zmultiset"
-  icaps :: "('nid, 'p) location \<Rightarrow> 't zmultiset"
-  cbufs :: "'nid \<Rightarrow> 'p \<Rightarrow> ('d \<times> 't) buf"
-  obufs :: "'nid \<Rightarrow> 'p \<Rightarrow> ('d \<times> 't) buf"
-  ibufs :: "'nid \<Rightarrow> 'p \<Rightarrow> ('d \<times> 't) buf"
-  logcs :: "'nid \<Rightarrow> (('p \<Rightarrow> 't antichain) \<Rightarrow> ('p \<Rightarrow> ('d \<times> 't) buf) \<Rightarrow> ('p \<Rightarrow> 't zmultiset) \<Rightarrow>
-                    ('p \<Rightarrow> ('d \<times> 't) buf) \<times> ('p \<Rightarrow> ('d \<times> 't) buf) \<times> ('p \<Rightarrow> 't zmultiset)) stream"
-
-abbreviation "dataplane_state ec ic cb ob ib lgc \<equiv> \<lparr>
-  ecaps = ec,
-  icaps = ic,
-  cbufs = cb,
-  obufs = ob,
-  ibufs = ib,
-  logcs = lgc
- \<rparr>"
-
-definition caps_report_action where
-  "caps_report_action ds ds' = 
-  (\<exists> l. ds' = ds\<lparr>ecaps := (ecaps ds)(l := ecaps ds l + icaps ds l), icaps := (icaps ds)(l := {#}\<^sub>z) \<rparr>)"
-
-definition consumes_action where
-  "consumes_action summary ds ds' = (\<exists> nid pfx sfx icaps' icaps''.
-   (\<forall> p. pfx p @ sfx p = cbufs ds nid p) \<and>
-   icaps' = (\<lambda> l. case l of Loc nid' (Trg p) \<Rightarrow> if nid = nid' then to_zmset (map snd (pfx p)) else {#}\<^sub>z | _ \<Rightarrow> {#}\<^sub>z) \<and>
-   icaps'' = (\<lambda> l'. sum (\<lambda> l. icaps' l -++- (summary l l')) UNIV) \<and>
-   ds' = ds\<lparr> 
-     cbufs := (cbufs ds)(nid := \<lambda> p. sfx p),
-     ibufs := (ibufs ds)(nid := \<lambda> p. ibufs ds nid p @ pfx p),
-     icaps := (\<lambda> l. icaps ds l - icaps' l + icaps'' l)
-    \<rparr>)"
-
-definition implied_frontier where
-  "implied_frontier summary caps loc = 
-  frontier (\<Sum>loc'\<in>UNIV. after_summary (dataflow_topology.zmset_frontier (caps loc')) (dataflow_topology.path_summary summary loc' loc))"
-declare implied_frontier_def[code del]
-
-definition "sound_output outs caps = (\<forall> p t d. (d, t) \<in> set (outs p) \<longrightarrow> zcount (caps p) t > 0)"
-
-definition "caps_to_location_Src nid caps l = (case l of Loc nid' (Src p) \<Rightarrow> if nid' = nid then caps p else {#}\<^sub>z | _ \<Rightarrow> {#}\<^sub>z)"
-
-lemma caps_to_location_Src_add_simp[simp]:
-  "caps_to_location_Src nid M1 l + caps_to_location_Src nid M2 l = 
-   caps_to_location_Src nid (\<lambda> p. M1 p + M2 p) l"
-  unfolding caps_to_location_Src_def
-  by (auto split: location.splits port.splits)
-
-lemma caps_to_location_Src_diff_location[simp]:
-  "nid \<noteq> node l \<Longrightarrow> caps_to_location_Src nid M l = {#}\<^sub>z"
-  unfolding caps_to_location_Src_def
-  by (auto split: location.splits port.splits)
-
-
-definition "outputs_to_internal_channels summary nid outs nid' p' =
-  (concat (map (\<lambda> p. if summary (Loc nid (Src p)) (Loc nid' (Trg p')) \<noteq> {}\<^sub>A then outs p else []) Enum.enum))"
-
-lemma outputs_to_internal_channels_empty_simp[simp]:
-  "outputs_to_internal_channels summary nid (\<lambda> _. []) = (\<lambda> _ _. [])"
-  unfolding outputs_to_internal_channels_def
-  apply force
-  done
-
-definition "outputs_to_visible_channels summary nid outs nid' p' =
-  (if nid = nid' \<and> (\<forall> l. summary (Loc nid' (Src p')) l = {}\<^sub>A) then outs p' else [])"
-
-lemma outputs_to_visible_channels_empty_simp[simp]:
-  "outputs_to_visible_channels summary nid (\<lambda> _. []) = (\<lambda> _ _. [])"
-  unfolding outputs_to_visible_channels_def
-  apply (rule ext)+
-  apply clarsimp
-  done
-
-
-
-definition produces_action where
-  "produces_action summary ds ds' = 
-  (\<exists> nid pfxbuf pfxbuf' sfxbuf outs  ccaps f imp_fron caps ccaps_l cbufs' obufs'.
-    f = shd (logcs ds nid) \<and>
-    (\<forall> p. pfxbuf p @ sfxbuf p = ibufs ds nid p) \<and>
-    caps = (\<lambda> p. icaps ds (Loc nid (Src p)) + ecaps ds (Loc nid (Src p))) \<and>
-    imp_fron = (\<lambda> p. implied_frontier summary (ecaps ds) (Loc nid (Trg p))) \<and>
-    (pfxbuf', outs, ccaps) = f imp_fron pfxbuf caps \<and> 
-    ccaps_l = caps_to_location_Src nid ccaps \<and>
-    cbufs' = outputs_to_internal_channels summary nid outs \<and>
-    obufs' = outputs_to_visible_channels summary nid outs \<and>
-    sound_output outs caps \<and>
-    ds' = ds\<lparr> 
-     ibufs := (ibufs ds)(nid := (\<lambda> p. pfxbuf' p @ sfxbuf p)),
-     icaps := (\<lambda> l. icaps ds l + ccaps_l l),
-     cbufs := (\<lambda> nid p. cbufs ds nid p @ cbufs' nid p),
-     logcs := (logcs ds)(nid := stl (logcs ds nid)),
-     obufs := (\<lambda> nid p. obufs ds nid p @ obufs' nid p)
-     \<rparr>)"
-
-definition timely_action where
-  "timely_action summary ds ds' =
-  (caps_report_action ds ds' \<or> consumes_action summary ds ds' \<or> produces_action summary ds ds')"
-
-coinductive timely_trace for summary where                                                                         
-  tt_silent[intro!]: 
-  "timely_action summary ds ds' \<Longrightarrow> timely_trace summary n ds' outs \<Longrightarrow> timely_trace summary (Suc n) ds outs"
-| tt_visible[intro!]: 
-  "outs (nid, p) = LCons x lxs \<Longrightarrow>
-   outs' = outs((nid, p) := lxs) \<Longrightarrow>
-   ds' = ds\<lparr> obufs := \<lambda> nid' p'. if nid' = nid \<and> p' = p then xs else obufs ds nid' p' \<rparr> \<Longrightarrow>
-   obufs ds nid p = x # xs \<Longrightarrow> timely_trace summary n ds' outs' \<Longrightarrow> timely_trace summary 0 ds outs"
-| tt_stop[intro!]:
-  "(\<forall> nid p. obufs ds nid p = []) \<Longrightarrow>timely_trace summary 0 ds outs"
-
-primcorec lgc_input where
-  "lgc_input inps = SCons (\<lambda> imp_fron pfxbuf caps.
-  (pfxbuf,
-    \<lambda> p. case inps p of LCons (Data t d) lxs \<Rightarrow> [(d, t)] | _ \<Rightarrow> [],
-    \<lambda> p. case inps p of
-       LCons (Mint t) lxs \<Rightarrow> {# t #}\<^sub>z
-     | LCons (Drop t) lxs \<Rightarrow> - {# t #}\<^sub>z
-     | LCons _ _ \<Rightarrow> {#}\<^sub>z
-     | LNil \<Rightarrow> - caps p )
-   ) (lgc_input (\<lambda> p. ltl (inps p)))"
-
-definition "my_max t pfxbuf = Max (set (map fst (filter (\<lambda> (d, t'). t = t') (pfxbuf 1))))"
-
-abbreviation "lgc_max \<equiv> sconst (\<lambda> imp_fron pfxbuf caps.
-    let below_caps = filter_zmset (\<lambda> t'. \<not> frontier_less_equal (imp_fron 1) t') (caps 1) in
-    let ts = rmdups {} (map snd (filter (\<lambda> (d, t). t \<in>#\<^sub>z below_caps) (pfxbuf 1))) in  (
-    \<lambda> p. filter (\<lambda> (d, t). t \<notin>#\<^sub>z below_caps) (pfxbuf 1),
-    \<lambda> p. map (\<lambda> t. (my_max t pfxbuf, t)) ts,
-    \<lambda> p. - below_caps )
-   )"
-
-abbreviation "DS \<equiv> dataplane_state (\<lambda> l. case l of Loc nid (Src p) \<Rightarrow> {# \<bottom> #}\<^sub>z | _ \<Rightarrow> {#}\<^sub>z) (\<lambda> _. {#}\<^sub>z) (\<lambda> _ _. []) (\<lambda> _ _. []) (\<lambda> _ _. []) (\<lambda> (nid :: 2). if nid = 0 then lgc_input (\<lambda> _ :: 1. inps2) else lgc_max)"
-
-definition "my_summ = (\<lambda> l1 l2.
-   if l1 = Loc (0 :: 2) (Src (0 :: 1)) \<and> l2 = Loc (1 :: 2)  (Trg (0 :: 1)) 
-   then antichain_from_list [\<bottom>]
-   else if l1 = Loc 0 (Trg 0) \<and> l2 = Loc 0 (Src 0)
-   then antichain_from_list [\<bottom>]
-   else if l1 = Loc 1 (Trg 0) \<and> l2 = Loc 1 (Src 0)
-   then antichain_from_list [\<bottom>]
-   else {}\<^sub>A)"
-
-
-lemma my_summ_simps[simp]:
-  "my_summ l l = {}\<^sub>A"
-  "my_summ (Loc 0 (Trg 1)) (Loc 0 (Src 1)) = antichain_from_list [\<bottom>]"
-  "my_summ (Loc 0 (Trg 1)) (Loc 1 (Trg 1)) = {}\<^sub>A"
-  "my_summ (Loc 0 (Trg 1)) (Loc 1 (Src 1)) = {}\<^sub>A"
-  "my_summ (Loc 0 (Src 1)) (Loc 1 (Trg 1)) = antichain_from_list [\<bottom>]"
-  "my_summ (Loc 1 (Trg 1)) (Loc 1 (Src 1)) = antichain_from_list [\<bottom>]"
-  unfolding my_summ_def
-       apply auto
-  done
-
-lemma path_weight_my_summ_simps[simp]:
-  "graph.path_weight my_summ l1 l2 = (
-   if l1 = Loc (0 :: 2) (Src (0 :: 1)) \<and> l2 = Loc (1 :: 2)  (Trg (0 :: 1)) 
-   then antichain_from_list [\<bottom>]
-   else if l1 = Loc 0 (Trg 0) \<and> l2 = Loc 0 (Src 0)
-   then antichain_from_list [\<bottom>]
-   else if l1 = Loc 1 (Trg 0) \<and> l2 = Loc 1 (Src 0)
-   then antichain_from_list [\<bottom>]
-   else if l1 = Loc 0 (Trg 0) \<and> l2 = Loc 1 (Trg 0)
-   then antichain_from_list [\<bottom>]
-   else if l1 = Loc 0 (Trg 0) \<and> l2 = Loc 1 (Src 0)
-   then antichain_from_list [\<bottom>]
-   else if l1 = Loc 0 (Src 0) \<and> l2 = Loc 1 (Src 0)
-   then antichain_from_list [\<bottom>]
-   else if l1 = l2
-   then antichain_from_list [\<bottom>]
-   else {}\<^sub>A)"
-  oops
-
-lemma implied_frontier_my_summ[simp]:
-  "implied_frontier my_summ caps (Loc 1 (Trg 1)) = 
-   frontier (dataflow_topology.zmset_frontier (caps (Loc 1 (Trg 1))) +
-   dataflow_topology.zmset_frontier (caps (Loc 0 (Src 1))) +
-   dataflow_topology.zmset_frontier (caps (Loc 0 (Trg 1))))"
-(*   unfolding implied_frontier_def
-  using loc_2_1_cases[where l=loc] apply -
-  apply (elim disjE)
-  subgoal
-    apply simp
- *)
-  sorry
-
-abbreviation "my_14 \<equiv> Suc (Suc (Suc (Suc (Suc (Suc (Suc (Suc (Suc (Suc (Suc (Suc (Suc (Suc 0)))))))))))))"
-
-lemma
-  "timely_trace my_summ my_14 DS (\<lambda> (nid, p). if nid = 0 then LNil else LCons (10, MyPair 1 1) (LCons (7, MyPair 0 1) (LCons (3, MyPair 1 0) LNil)))"
-  apply (rule tt_silent)
-  unfolding timely_action_def
-   apply (rule disjI2)+
-  unfolding produces_action_def
-   apply (rule exI[of _ 0])
-   apply (rule exI[of _ "\<lambda> _. []"])
-   apply (rule exI[of _ "\<lambda> _. []"])
-   apply (rule exI[of _ "\<lambda> _. []"])
-   apply (rule exI[of _ "\<lambda> _. []"])
-   apply (rule exI[of _ "\<lambda> _. {# t_1_0 #}\<^sub>z"])
-   apply clarsimp
-  apply (simp add: sound_output_def)
-
-  apply (rule tt_silent)
-  unfolding timely_action_def
-   apply (rule disjI2)+
-  unfolding produces_action_def
-   apply (rule exI[of _ 0])
-   apply (rule exI[of _ "\<lambda> _. []"])
-   apply (rule exI[of _ "\<lambda> _. []"])
-   apply (rule exI[of _ "\<lambda> _. []"])
-   apply (rule exI[of _ "\<lambda> _. []"])
-   apply (rule exI[of _ "\<lambda> _. {# t_0_1 #}\<^sub>z"])
-  apply (simp add: sound_output_def)
-
-  apply (rule tt_silent)
-  unfolding timely_action_def
-   apply (rule disjI2)+
-  unfolding produces_action_def
-   apply (rule exI[of _ 0])
-   apply (rule exI[of _ "\<lambda> _. []"])
-   apply (rule exI[of _ "\<lambda> _. []"])
-   apply (rule exI[of _ "\<lambda> _. []"])
-   apply (rule exI[of _ "\<lambda> _. []"])
-   apply (rule exI[of _ "\<lambda> _. {# t_1_1 #}\<^sub>z"])
-    apply (simp add: sound_output_def)
-
-
-  apply (rule tt_silent)
-  unfolding timely_action_def
-   apply (rule disjI2)+
-  unfolding produces_action_def
-   apply (rule exI[of _ 0])
-   apply (rule exI[of _ "\<lambda> _. []"])
-   apply (rule exI[of _ "\<lambda> _. []"])
-   apply (rule exI[of _ "\<lambda> _. []"])
-   apply (rule exI[of _ "\<lambda> _. []"])
-   apply (rule exI[of _ "\<lambda> _. - {# t0 #}\<^sub>z"])
-  apply (simp add: sound_output_def)
-
-  apply (rule tt_silent)
-  unfolding timely_action_def
-   apply (rule disjI2)+
-  unfolding produces_action_def
-  apply (rule exI[of _ 0])
-   apply (intro exI conjI)
-            apply (rule refl)+
-           apply simp
-          apply (rule refl)+
-        apply simp
-       apply simp
-      apply (rule refl)+
-  subgoal
-    unfolding sound_output_def
-    apply simp
-    apply code_simp
-    done
-      apply (rule refl)+
-
-
-  apply (rule tt_silent)
-  unfolding timely_action_def
-   apply (rule disjI2)+
-  unfolding produces_action_def
-  apply (rule exI[of _ 0])
-   apply (intro exI conjI)
-            apply (rule refl)+
-           apply simp
-          apply (rule refl)+
-        apply simp
-       apply simp
-      apply (rule refl)+
-  subgoal
-    unfolding sound_output_def
-    apply simp
-    done
-   apply (rule refl)+
-  apply simp
-
-  apply (rule tt_silent)
-  unfolding timely_action_def
-   apply (rule disjI2)+
-  unfolding produces_action_def
-   apply (rule exI[of _ 0])
-   apply (intro exI conjI)
-            apply (rule refl)+
-           apply simp
-          apply (rule refl)+
-        apply simp
-       apply simp
-      apply (rule refl)+
-  subgoal
-    unfolding sound_output_def
-    apply simp
-    apply code_simp
-    done
-   apply (rule refl)+
-  apply simp
-
-  apply (rule tt_silent)
- unfolding timely_action_def
-   apply (rule disjI2)+
-  unfolding produces_action_def
-   apply (rule exI[of _ 0])
-   apply (intro exI conjI)
-            apply (rule refl)+
-           apply simp
-          apply (rule refl)+
-        apply simp
-       apply simp
-      apply (rule refl)+
-  subgoal
-    unfolding sound_output_def
-    apply simp
-    apply code_simp
-    done
-   apply (rule refl)+
-  apply clarsimp
-
- apply (rule tt_silent)
- unfolding timely_action_def
-   apply (rule disjI2)+
-  unfolding produces_action_def
-   apply (rule exI[of _ 0])
-   apply (intro exI conjI)
-            apply (rule refl)+
-           apply simp
-          apply (rule refl)+
-        apply simp
-       apply simp
-      apply (rule refl)+
-  subgoal
-    unfolding sound_output_def
-    apply simp
-    done
-   apply (rule refl)+
-  apply clarsimp
-
- apply (rule tt_silent)
- unfolding timely_action_def
-   apply (rule disjI2)+
-  unfolding produces_action_def
-   apply (rule exI[of _ 0])
-   apply (intro exI conjI)
-            apply (rule refl)+
-           apply simp
-          apply (rule refl)+
-        apply simp
-       apply simp
-      apply (rule refl)+
-  subgoal
-    unfolding sound_output_def
-    apply simp
-    done
-   apply (rule refl)+
-  apply clarsimp
-
- apply (rule tt_silent)
-  unfolding timely_action_def
-   apply (rule disjI1)
-  unfolding caps_report_action_def
-   apply (rule exI[of _ "Loc 0 (Src 1)"])
-   apply simp
-
- apply (rule tt_silent)
-  unfolding timely_action_def
-   apply (rule disjI2)
-   apply (rule disjI1)
-  unfolding consumes_action_def
-   apply (rule exI[of _ 1])
-   apply (rule exI[of _ "\<lambda> _. [(10, t_1_1), (7, t_0_1), (3, t_1_0)]"])
-  apply (rule exI[of _ "\<lambda> _. []"])
-   apply (intro exI conjI)
-      apply (clarsimp simp add: outputs_to_internal_channels_def)
-      apply (intro conjI impI)
-  subgoal
-    unfolding antichain_from_list_antichain antichain_from_list_is_empty my_summ_def
-    apply simp
-    apply (subst (asm) antichain_not_empty)
-      apply (auto simp add: incomparable_def)
-    done
-  subgoal premises
-    by code_simp
-  apply (rule refl)+
-  apply simp
-
- apply (rule tt_silent)
-  unfolding timely_action_def
-   apply (rule disjI1)
-  unfolding caps_report_action_def
-   apply (rule exI[of _ "Loc 1 (Trg 1)"])
-   apply (rule refl)
-  apply simp
-
-  apply (rule tt_silent)
- unfolding timely_action_def
-  apply (rule disjI2)+
-  unfolding produces_action_def
-   apply (rule exI[of _ 1])
-   apply (rule exI[of _ "\<lambda> _. [(10, t_1_1), (7, t_0_1), (3, t_1_0)]"])
-   apply (rule exI[of _ "\<lambda> _. []"])
-   apply (rule exI[of _ "\<lambda> _. []"])
-   apply (rule exI[of _ "\<lambda> _. [(10, t_1_1), (7, t_0_1), (3, t_1_0)]"])
-   apply (rule exI[of _ "\<lambda> _. - {# t_1_1, t_0_1, t_1_0, t0 #}\<^sub>z"])
-   apply (intro exI conjI)
-            apply (rule refl)+
-           apply simp
-          apply (rule refl)+
-  subgoal
-    apply (simp only: prod_eq_iff)
-    subgoal
-      apply (simp add: neg_neg_multiset caps_to_location_Src_def)
-      apply (simp add: my_max_def caps_to_location_Src_def uminus_add_zmset add_del_zmset weird_singleton)
-      done
-    done
-              apply (rule refl)+
-  subgoal
-    unfolding sound_output_def my_summ_def
-    apply (auto simp add: weird_singleton split: location.splits)
-    done
-              apply (rule refl)+
-  apply simp
-  apply (rule tt_visible[where p=1 and nid=1])
-      apply simp
-  apply (rule refl)+
-   apply (simp add: outputs_to_visible_channels_def my_summ_def)
-
-  apply (rule tt_visible[where p=1 and nid=1])
-      apply simp
-  apply (rule refl)+
-   apply (simp add: outputs_to_visible_channels_def my_summ_def)
-
-  apply (rule tt_visible[where p=1 and nid=1])
-      apply simp
-  apply (rule refl)+
-   apply (simp add: outputs_to_visible_channels_def my_summ_def)
-
-  apply (rule tt_stop)
-  apply (intro impI allI conjI)
-  apply simp
-  apply (intro impI allI conjI)
-  defer
-      apply (auto simp add: antichain_from_list_antichain weird_singleton outputs_to_visible_channels_def my_summ_def)[1]
-  apply (metis empty_antichain.rep_eq insert_not_empty set_antichain_antichain_singleton)
-      apply (auto simp add: antichain_from_list_antichain weird_singleton outputs_to_visible_channels_def my_summ_def)[1]
-  apply (metis empty_antichain.rep_eq insert_not_empty set_antichain_antichain_singleton)
-      apply (auto simp add: outputs_to_visible_channels_def antichain_from_list_antichain weird_singleton my_summ_def)
-  apply (metis empty_antichain.rep_eq insert_not_empty set_antichain_antichain_singleton)
-  done
-
-lemma
-  assumes \<open>(x, t) \<in> lset (outs (1, 1))\<close>
-  and \<open>SM = dataplane_state ec ic cb ob ib (\<lambda> (nid :: 2). if nid = 0 then lgc_input (\<lambda> _ :: 1. inps) else lgc_max)\<close>
-  and \<open>ob = (\<lambda> nid p. if nid = 1 \<and> p = 1 then ob1 else [])\<close>
-  and \<open>timely_trace my_summ n SM outs\<close>
-obtains \<open>x \<in> (Data t) -` lset (map (\<lambda> (d, t). Data t d) (ib 1 1) @@- map (\<lambda> (d, t). Data t d) (cb 1 1) @@- inps)\<close> | \<open>(x, t) \<in> set ob1\<close>
-  using assms apply -
-  apply hypsubst_thin
-  apply atomize_elim
-    apply (induct "outs (1, 1)" rule: lset_induct)
-  subgoal for lxs
-    apply (drule sym)
-      apply simp
-      apply (induct n)
-      apply simp_all
-    subgoal
-      apply (erule timely_trace.cases)
-        apply simp_all
-      subgoal for outsa nid xa lxsa outs' ds' xs ds n
-        apply hypsubst_thin
-        apply (rule disjI2)+
-        apply (metis (mono_tags, lifting) dataplane_state.simps(4) list.distinct(1) list.set_intros(1) llist.inject)
-        done
-      subgoal for ds outs'
-        apply hypsubst_thin
-
-  find_theorems lset lnth
-
-end
-
-term "[Mint t_1_0, Mint t_0_1, Mint t_1_1, Drop t0, Data t_1_1 10, Drop t_1_1, Data t_0_1 7, Data t_1_0 (3 :: nat), Drop t_1_0, Drop t_0_1]"
 
 abbreviation init_input_state where
 "init_input_state su inps \<equiv> \<lparr> 
@@ -604,27 +62,40 @@ abbreviation "test_dt2 \<equiv> Comp [(0, 1) \<mapsto> (0, 1)] (l1 (\<lambda> _.
 
 abbreviation "test_op2 \<equiv> compile_dataflow test_dt2 :: (2 \<times> 1, 2 \<times> 1, _) op"
 
+abbreviation "set_op_test \<equiv> set_op {||} {||} test_op2"
 
-term Set.the_elem
+
 (* 
 value [GHC] "lmap (\<lambda> io. case io of VOut p (x, t) \<Rightarrow> (projr x, t)) (trace_exec test_op1)"
  *)
-value r1
 
-value [GHC] "crmdups id {|Suc 0, Suc 0|}"
+find_theorems cUn name: code
 
 
-definition "my_test =  (trace_exec test_op2)"
-
-value [GHC] my_test
-
+value [GHC] "trace_exec set_op_test"
 
 value "frontier {# t_1_1, t_0_1, t_1_0 #}\<^sub>z"
 
 term DEBUG
 
-definition "looping = check_prefix [VOut (1, 1) (Inr 3, MyPair 1 0)] test_op2"
+find_theorems Max fold
 
+abbreviation "timestamps inps \<equiv> cset_of_llist (lmap (\<lambda> ev. case ev of Data t d \<Rightarrow> t) (lfilter is_Data inps))"
+
+abbreviation "Max_spec inps \<equiv> 
+  cimage (\<lambda> t. (1 :: 1, Max (set (list_of (lmap (\<lambda> ev. case ev of Data _ d \<Rightarrow> d) (lfilter (\<lambda> ev. case ev of Data t' d \<Rightarrow> t = t' | _ \<Rightarrow> False) inps)))), t))
+  (timestamps inps)"
+
+value [GHC] "(Max_spec inps2)"
+
+value [GHC] "trace_exec (set_op (Max_spec inps2) {||} (\<oslash> :: (1, _, _) op))"
+
+value [GHC] "check_prefix [VOut 1 (3, MyPair 1 0)] (set_op (Max_spec inps2) {||} (\<oslash> :: (1, _, _) op))"
+
+value [GHC] "check_prefix [VOut (1, 1) (Inr 3, MyPair 1 0)] set_op_test"
+
+
+end
  (* 
 value [GHC] "check_prefix [VOut (1, 1) (Inr 10, MyPair 1 1)] test_op2"
  *)
@@ -634,9 +105,7 @@ value [GHC] "check_prefix [VOut (1, 1) (Inr 7, MyPair 0 1)] test_op2"
 value [GHC] "check_prefix [VOut (1, 1) (Inr 3, MyPair 1 0)] test_op2"
  *)
 
-value [GHC] "trace_exec spec_op_test"
 
-print_classes
 
 (* 
 value [GHC] "check_prefix [VOut 1 (7, MyPair 0 1)] spec_op_test"
@@ -655,11 +124,16 @@ value [GHC] "check_prefix [VOut 1 (10, MyPair 1 1)] spec_op_test"
 (* value [GHC] "approx_in 30 [VOut (1, 1) (Inr 3, MyPair 1 0)] test_op2"
 
  *)
-term DEBUG
 
-thm cUnion_code
 
-term cUn
+
+lemma
+  "set_op S S' test_op2 \<approx> set_op (cUn S A) S' \<oslash>"
+  oops
+
+lemma
+  "set_op {||} {||} test_op2 \<approx> set_op A {||} \<oslash>"
+
 end
 
 abbreviation "inp_op os \<equiv> map_op (case_option (Inl (0 :: 2)) (\<lambda> p. Inr (0, p))) (case_option (Inl (0 :: 2)) (\<lambda> p. Inr (0, p))) (ooo_input_op {|1|} os)"
