dataplane/Examples/Set_op.thy
@@ -1,0 +1,26 @@
+theory Set_op
+
+imports
+  Nondeterministic_Dataflow.Operator
+begin
+
+corec set_op :: "('a \<times> 'b) cset \<Rightarrow> ('a \<times> 'b) cset \<Rightarrow> ('c, 'a, 'b) op \<Rightarrow> ('c, 'a, 'b) op" where
+  "set_op S S' op = choice2
+  (Choice (cimage (\<lambda> op. case op of
+     Write op p x \<Rightarrow> Silent (set_op (cinsert (p, x) S) S' op) 
+   | Silent op \<Rightarrow> Silent (set_op S S' op)
+   | Read _ _ \<Rightarrow> Code.abort (STR ''Set_op can only output'') (\<lambda> _. \<oslash>)
+   ) (choices op))
+  
+   )
+  (Choice (cimage (\<lambda> (p, x). Write (set_op S (cinsert (p, x) S') op) p x) (S - S')))"
+  
+
+(* lemma
+  "wtraces (set_op op) = (wtraces op)"
+  unfolding wtraces_def
+  apply auto
+  subgoal for vios
+    oops
+ *)
+end
